imp almost done

Imp.v
@@ -238,3 +238,490 @@ Inductive aevalR : aexp -> nat -> Prop :=
       (e1 \\ n1) -> (e2 \\ n2) 
    -> (AMult e1 e2) \\ (n1 * n2)
   where "e '\\' n" := (aevalR e n) : type_scope.
+
+Theorem aeval_iff_aevalR : forall a n,
+  (a \\ n) <-> aeval a = n.
+Proof.
+  split.
+  - intros H. induction H; simpl.
+    + (* E_ANum *)
+      reflexivity.
+    + (* E_APlus *)
+      rewrite IHaevalR1. rewrite IHaevalR2. reflexivity.
+    + (* E_AMinus *)
+      rewrite IHaevalR1. rewrite IHaevalR2. reflexivity.
+    + (* E_AMult *)
+      rewrite IHaevalR1. rewrite IHaevalR2. reflexivity.
+  - generalize dependent n. induction a;
+    simpl; intros; subst.
+    + apply E_ANum.
+    + apply E_APlus.
+      apply IHa1. reflexivity.
+      apply IHa2. reflexivity.
+    + (* AMinus *)
+      apply E_AMinus.
+      apply IHa1. reflexivity.
+      apply IHa2. reflexivity.
+    + (* AMult *)
+      apply E_AMult.
+      apply IHa1. reflexivity.
+      apply IHa2. reflexivity.
+Qed.
+ 
+Theorem aeval_iff_aevalR' : forall a n,
+  (a \\ n) <-> aeval a = n.
+Proof.
+  split.
+  - intros H; induction H; 
+    try (subst; reflexivity).
+  - generalize dependent n.
+    induction a; simpl; intros; subst; 
+    constructor; try apply IHa1; 
+    try apply IHa2; reflexivity.
+Qed.
+
+Lemma aeval_a_aevalR : forall e,
+  e \\ aeval e.
+Proof.
+  intros.
+  apply aeval_iff_aevalR' with (a := e) (n := (aeval e)).
+  reflexivity.
+Qed.
+
+Reserved Notation "e '//' n" 
+  (at level 90, left associativity).
+Inductive bevalR : bexp -> bool -> Prop :=
+  | E_BTrue : BTrue // true
+  | E_BFalse : BFalse // false
+  | E_BEq (e1 e2 : aexp) (n1 n2 : nat) (b : bool):
+      (e1 \\ n1) -> (e2 \\ n2) -> 
+        b = (n1 =? n2) ->
+          (BEq e1 e2) // b
+  | E_BLe (e1 e2 : aexp) (n1 n2 : nat) (b : bool):
+      (e1 \\ n1) -> (e2 \\ n2) -> 
+        b = (n1 <=? n2) ->
+          (BLe e1 e2) // b
+  | E_BNot (e1 : bexp) (b : bool) :
+      (e1 // b) -> (BNot e1) // (negb b) 
+  | E_BAnd (e1 e2 : bexp) (b1 b2 : bool) :
+      (e1 // b1) -> (e2 // b2) ->
+        (BAnd e1 e2) // (b1 && b2)
+  where "e '//' n" := (bevalR e n) : type_scope.
+
+Lemma beval_iff_bevalR : forall b bv,
+  bevalR b bv <-> beval b = bv.
+Proof.
+  split.
+  - intros H. induction H; simpl; try reflexivity;
+    try (apply aeval_iff_aevalR in H; 
+         apply aeval_iff_aevalR in H0;
+         subst; reflexivity).
+    + rewrite IHbevalR. reflexivity.
+    + rewrite IHbevalR1, IHbevalR2. reflexivity.
+  - generalize dependent bv. 
+    induction b; simpl; intros.
+    + subst. constructor.
+    + subst. constructor.
+    + apply E_BEq with (n1 := aeval a1) (n2 := aeval a2).
+      apply aeval_a_aevalR. apply aeval_a_aevalR. 
+      rewrite H. reflexivity.
+    + apply E_BLe with (n1 := aeval a1) (n2 := aeval a2).
+      apply aeval_a_aevalR. apply aeval_a_aevalR. 
+      rewrite H. reflexivity.
+    + rewrite <- H. constructor.
+      apply IHb. reflexivity.
+    + rewrite <- H. constructor.
+      apply IHb1. reflexivity. apply IHb2. reflexivity.
+Qed.
+
+End AExp.
+
+Module aevalR_division.
+
+Inductive aexp : Type :=
+  | ANum (n : nat)
+  | APlus (a1 a2 : aexp)
+  | AMinus (a1 a2 : aexp)
+  | AMult (a1 a2 : aexp)
+  | ADiv (a1 a2 : aexp). (* <--- NEW *)
+
+Reserved Notation "e '\\' n" (at level 90, left associativity).
+Inductive aevalR : aexp -> nat -> Prop :=
+  | E_ANum (n : nat) : (ANum n) \\ n
+  | E_APlus (e1 e2 : aexp) (n1 n2 : nat) :
+      (e1 \\ n1) -> (e2 \\ n2) 
+   -> (APlus e1 e2) \\ (n1 + n2)
+  | E_AMinus (e1 e2 : aexp) (n1 n2 : nat) :
+      (e1 \\ n1) -> (e2 \\ n2) 
+   -> (AMinus e1 e2) \\ (n1 - n2)
+  | E_AMult (e1 e2 : aexp) (n1 n2 : nat) :
+      (e1 \\ n1) -> (e2 \\ n2) 
+   -> (AMult e1 e2) \\ (n1 * n2)
+  | E_ADiv (a1 a2 : aexp) (n1 n2 n3 : nat) :
+      (a1 \\ n1) -> (a2 \\ n2) -> (n2 > 0) ->
+      (mult n2 n3 = n1) -> (ADiv a1 a2) \\ n3
+  where "e '\\' n" := (aevalR e n) : type_scope.
+End aevalR_division.
+
+Module aevalR_extended.
+
+Reserved Notation "e '\\' n" (at level 90, left associativity).
+Inductive aexp : Type :=
+  | AAny (* <--- NEW *)
+  | ANum (n : nat)
+  | APlus (a1 a2 : aexp)
+  | AMinus (a1 a2 : aexp)
+  | AMult (a1 a2 : aexp).
+
+Reserved Notation "e '\\' n" (at level 90, left associativity).
+Inductive aevalR : aexp -> nat -> Prop :=
+  | E_Any (n : nat) :
+      AAny \\ n (* <--- NEW *)
+  | E_ANum (n : nat) : (ANum n) \\ n
+  | E_APlus (e1 e2 : aexp) (n1 n2 : nat) :
+      (e1 \\ n1) -> (e2 \\ n2) 
+   -> (APlus e1 e2) \\ (n1 + n2)
+  | E_AMinus (e1 e2 : aexp) (n1 n2 : nat) :
+      (e1 \\ n1) -> (e2 \\ n2) 
+   -> (AMinus e1 e2) \\ (n1 - n2)
+  | E_AMult (e1 e2 : aexp) (n1 n2 : nat) :
+      (e1 \\ n1) -> (e2 \\ n2) 
+   -> (AMult e1 e2) \\ (n1 * n2)
+  where "e '\\' n" := (aevalR e n) : type_scope.
+
+End aevalR_extended.
+
+Definition state := total_map nat.
+
+Inductive aexp : Type :=
+  | ANum (n : nat)
+  | AId (x : string) (* <--- NEW *)
+  | APlus (a1 a2 : aexp)
+  | AMinus (a1 a2 : aexp)
+  | AMult (a1 a2 : aexp).
+
+Definition W : string := "W".
+Definition X : string := "X".
+Definition Y : string := "Y".
+Definition Z : string := "Z".
+
+Inductive bexp : Type :=
+  | BTrue
+  | BFalse
+  | BEq (a1 a2 : aexp)
+  | BLe (a1 a2 : aexp)
+  | BNot (b : bexp)
+  | BAnd (b1 b2 : bexp).
+
+Coercion AId : string >-> aexp.
+Coercion ANum : nat >-> aexp.
+
+Definition bool_to_bexp (b : bool) : bexp :=
+  if b then BTrue else BFalse.
+Coercion bool_to_bexp : bool >-> bexp.
+
+Bind Scope imp_scope with aexp.
+Bind Scope imp_scope with bexp.
+Delimit Scope imp_scope with imp.
+
+Notation "x + y" := (APlus x y) (at level 50, left associativity) : imp_scope.
+Notation "x - y" := (AMinus x y) (at level 50, left associativity) : imp_scope.
+Notation "x * y" := (AMult x y) (at level 40, left associativity) : imp_scope.
+Notation "x ≤ y" := (BLe x y) (at level 70, no associativity) : imp_scope.
+Notation "x = y" := (BEq x y) (at level 70, no associativity) : imp_scope.
+Notation "x && y" := (BAnd x y) (at level 40, left associativity) : imp_scope.
+Notation "'~' b" := (BNot b) (at level 75, right associativity) : imp_scope.
+
+Definition example_aexp := (3 + (X * 2))%imp : aexp.
+Definition example_bexp := (true && ~ (X ≤ 4))%imp : bexp.
+
+Set Printing Coercions.
+
+Print example_bexp.
+
+Unset Printing Coercions.
+
+Fixpoint aeval (st : state) (a : aexp) : nat :=
+  match a with
+  | ANum n => n
+  | AId x => st x
+  | APlus a1 a2 => (aeval st a1) + (aeval st a2)
+  | AMinus a1 a2 => (aeval st a1) - (aeval st a2)
+  | AMult a1 a2 => (aeval st a1) * (aeval st a2)
+  end.
+
+Fixpoint beval (st : state) (b : bexp) : bool :=
+  match b with
+  | BTrue => true
+  | BFalse => false
+  | BEq a1 a2 => (aeval st a1) =? (aeval st a2)
+  | BLe a1 a2 => (aeval st a1) <=? (aeval st a2)
+  | BNot b1 => negb (beval st b1)
+  | BAnd b1 b2 => andb (beval st b1) (beval st b2)
+  end.
+
+Definition empty_st := (_ !-> 0).
+Notation "a '!->' x" := (t_update empty_st a x) (at level 100).
+
+Example aexp1 :
+    aeval (X !-> 5) (3 + (X * 2))%imp
+  = 13.
+Proof. reflexivity. Qed.
+
+Example bexp1 :
+    beval (X !-> 5) (true && ~(X ≤ 4))%imp
+  = true.
+Proof. reflexivity. Qed.
+
+ Inductive com : Type :=
+  | CSkip
+  | CAss (x : string) (a : aexp)
+  | CSeq (c1 c2 : com)
+  | CIf (b : bexp) (c1 c2 : com)
+  | CWhile (b : bexp) (c : com).
+
+Bind Scope imp_scope with com.
+Notation "'SKIP'" :=
+   CSkip : imp_scope.
+Notation "x '::=' a" :=
+  (CAss x a) (at level 60) : imp_scope.
+Notation "c1 ;; c2" :=
+  (CSeq c1 c2) (at level 80, right associativity) : imp_scope.
+Notation "'WHILE' b 'DO' c 'END'" :=
+  (CWhile b c) (at level 80, right associativity) : imp_scope.
+Notation "'TEST' c1 'THEN' c2 'ELSE' c3 'FI'" :=
+  (CIf c1 c2 c3) (at level 80, right associativity) : imp_scope.
+
+Definition fact_in_coq : com :=
+  (Z ::= X;;
+  Y ::= 1;;
+  WHILE ~(Z = 0) DO
+    Y ::= Y * Z;;
+    Z ::= Z - 1
+  END)%imp.
+
+Unset Printing Notations.
+Print fact_in_coq.
+
+Locate "&&".
+Locate ";;".
+Locate "WHILE".
+
+Locate aexp.
+
+Definition plus2 : com :=
+  X ::= X + 2.
+Definition XtimesYinZ : com :=
+  Z ::= X * Y.
+Definition subtract_slowly_body : com :=
+  Z ::= Z - 1 ;;
+  X ::= X - 1.
+
+Definition subtract_slowly : com :=
+  (WHILE ~(X = 0) DO
+    subtract_slowly_body
+  END)%imp.
+
+Definition subtract_3_from_5_slowly : com :=
+  X ::= 3 ;;
+  Z ::= 5 ;;
+  subtract_slowly.
+
+Print subtract_slowly.
+
+Definition loop : com :=
+  WHILE true DO
+    SKIP
+  END.
+
+Open Scope imp_scope.
+Fixpoint ceval_fun_no_while (st : state) (c : com)
+                          : state :=
+  match c with
+    | SKIP => st
+    | x ::= a1 =>
+        (x !-> (aeval st a1) ; st)
+    | c1 ;; c2 =>
+        let st' := ceval_fun_no_while st c1 in
+          ceval_fun_no_while st' c2
+    | TEST b THEN c1 ELSE c2 FI =>
+        if (beval st b)
+          then ceval_fun_no_while st c1
+          else ceval_fun_no_while st c2
+    | WHILE b DO c END =>
+        st (* bogus *)
+  end.
+Close Scope imp_scope.
+
+Reserved Notation "st '=[' c ']=>' st'"
+                  (at level 40).
+
+Inductive ceval : com -> state -> state -> Prop :=
+  | E_Skip : forall st,
+      st =[ SKIP ]=> st
+  | E_Ass : forall st a1 n x,
+      aeval st a1 = n ->
+      st =[ x ::= a1 ]=> (x !-> n ; st)
+  | E_Seq : forall c1 c2 st st' st'',
+      st =[ c1 ]=> st' ->
+      st' =[ c2 ]=> st'' ->
+      st =[ c1 ;; c2 ]=> st''
+  | E_IfTrue : forall st st' b c1 c2,
+      beval st b = true ->
+      st =[ c1 ]=> st' ->
+      st =[ TEST b THEN c1 ELSE c2 FI ]=> st'
+  | E_IfFalse : forall st st' b c1 c2,
+      beval st b = false ->
+      st =[ c2 ]=> st' ->
+      st =[ TEST b THEN c1 ELSE c2 FI ]=> st'
+  | E_WhileFalse : forall b st c,
+      beval st b = false ->
+      st =[ WHILE b DO c END ]=> st
+  | E_WhileTrue : forall st st' st'' b c,
+      beval st b = true ->
+      st =[ c ]=> st' ->
+      st' =[ WHILE b DO c END ]=> st'' ->
+      st =[ WHILE b DO c END ]=> st''
+  where "st =[ c ]=> st'" := (ceval c st st').
+
+Example ceval_example1:
+  empty_st =[
+     X ::= 2;;
+     TEST X ≤ 1
+       THEN Y ::= 3
+       ELSE Z ::= 4
+     FI
+  ]=> (Z !-> 4 ; X !-> 2).
+Proof.
+  apply E_Seq with (X !-> 2).
+  - apply E_Ass. reflexivity.
+  - apply E_IfFalse. reflexivity.
+    apply E_Ass. reflexivity.
+Qed.
+
+Example ceval_example2:
+  empty_st =[
+    X ::= 0;; Y ::= 1;; Z ::= 2
+  ]=> (Z !-> 2 ; Y !-> 1 ; X !-> 0).
+Proof.
+  apply E_Seq with (X !-> 0).
+  - apply E_Ass. reflexivity.
+  - apply E_Seq with (Y !-> 1; X !-> 0);
+    apply E_Ass; reflexivity.
+Qed.
+
+Definition pup_to_n : com :=
+  (Y ::= 0;;
+  WHILE ~ (X = 0) DO
+    Y ::= X + Y ;;
+    X ::= X - 1
+   END) % imp.
+
+Theorem pup_to_2_ceval :
+  (X !-> 2) =[
+    pup_to_n
+  ]=> (X !-> 0 ; Y !-> 3 ; X !-> 1 ; Y !-> 2 ; Y !-> 0 ; X !-> 2).
+Proof.
+  unfold pup_to_n.
+  apply E_Seq with (Y !-> 0; X !-> 2).
+  - apply E_Ass. reflexivity.
+  - apply E_WhileTrue with (X !-> 1; Y !-> 2; Y !-> 0; X !-> 2).
+    + reflexivity.
+    + apply E_Seq with (Y !-> 2; Y !-> 0; X !-> 2);
+      apply E_Ass; reflexivity.
+    + apply E_WhileTrue with 
+      (X !-> 0; Y !-> 3; X !-> 1; Y !-> 2; Y !-> 0; X !-> 2).
+      * reflexivity.
+      * apply E_Seq with 
+          (Y !-> 3; X !-> 1; Y !-> 2; Y !-> 0; X !-> 2);
+        apply E_Ass; reflexivity.
+      * apply E_WhileFalse. reflexivity.
+Qed.
+
+Theorem ceval_deterministic: forall c st st1 st2,
+  st =[ c ]=> st1 ->
+  st =[ c ]=> st2 ->
+  st1 = st2.
+Proof.
+  intros c st st1 st2 E1 E2.
+  generalize dependent st2.
+  induction E1; intros st2 E2; inversion E2; subst.
+  - reflexivity.
+  - reflexivity.
+  - assert (st' = st'0) as EQ1.
+    { apply IHE1_1; assumption. }
+    subst st'0. apply IHE1_2. assumption.
+  - apply IHE1, H6.
+  - rewrite H in H5. discriminate H5.
+  - rewrite H in H5. discriminate H5.
+  - apply IHE1, H6.
+  - reflexivity.
+  - rewrite H in H2. discriminate H2.
+  - rewrite H in H4. discriminate H4.
+  - assert (st' = st'0) as EQ1.
+    { apply IHE1_1, H3. }
+    subst st'0. apply IHE1_2. assumption.
+Qed.
+
+Theorem plus2_spec : forall st n st',
+  st X = n ->
+  st =[ plus2 ]=> st' ->
+  st' X = n + 2.
+Proof.
+  intros st n st' HX Heval.
+  inversion Heval. subst. clear Heval. simpl.
+  apply t_update_eq.
+Qed.
+
+Theorem loop_never_stops : forall st st',
+  ~ (st =[ loop ]=> st').
+Proof.
+  intros st st' contra. unfold loop in contra.
+  remember (WHILE true DO SKIP END)%imp as loopdef 
+    eqn:Heqloopdef.
+  induction contra; try inversion Heqloopdef.
+  - rewrite H1 in H. simpl in H. discriminate H.
+  - subst. apply IHcontra2. reflexivity.
+Qed.
+
+Open Scope imp_scope.
+Fixpoint no_whiles (c : com) : bool :=
+  match c with
+  | SKIP =>
+      true
+  | _ ::= _ =>
+      true
+  | c1 ;; c2 =>
+      andb (no_whiles c1) (no_whiles c2)
+  | TEST _ THEN ct ELSE cf FI =>
+      andb (no_whiles ct) (no_whiles cf)
+  | WHILE _ DO _ END =>
+      false
+  end.
+Close Scope imp_scope.
+
+Inductive no_whilesR : com -> Prop :=
+  | N_Skip : no_whilesR SKIP
+  | N_Ass : forall x a,
+      no_whilesR (x ::= a)
+  | N_Seq : forall c1 c2,
+      no_whilesR c1 -> no_whilesR c2 ->
+      no_whilesR (c1 ;; c2)
+  | N_Test : forall b c1 c2,
+      no_whilesR c1 -> no_whilesR c2 ->
+        no_whilesR (TEST b THEN c1 ELSE c2 FI).
+
+Theorem no_whiles_eqv:
+   forall c, no_whiles c = true <-> no_whilesR c.
+Proof.
+  split. 
+  - intros. induction c;
+    try (simpl in H; apply andb_true_iff in H as [H H0]);
+    try constructor; try apply IHc1, H; try apply IHc2;
+    try apply H0. inversion H.
+  - intros H. induction c;
+    try reflexivity; try inversion H;
+    try (simpl; apply andb_true_iff; split);
+    try apply IHc1, H2; try apply IHc2; try apply H3;
+    try apply H4.
+Qed.
